Test/og/Program4.bpl
@@ -15,7 +15,7 @@ function {:inline} {:linear "tid"} TidSetCollector(x: [Tid]bool) : [Tid]bool
 
 var {:layer 0,1} a:[Tid]int;
 
-procedure Allocate() returns ({:linear "tid"} tid:Tid); 
+procedure {:yields} {:layer 1} Allocate() returns ({:linear "tid"} tid:Tid); 
 
 procedure {:yields} {:layer 1} main() { 
     var {:linear "tid"} tid:Tid;
