Test/og/parallel2.bpl
@@ -8,7 +8,7 @@ function {:inline} {:linear "tid"} TidCollector(x: int) : [int]bool
   MapConstBool(false)[x := true]
 }
 
-procedure Allocate() returns ({:linear "tid"} xls: int);
+procedure {:yields} {:layer 1} Allocate() returns ({:linear "tid"} xls: int);
 
 procedure {:yields} {:layer 0,1} Write(idx: int, val: int);
 ensures {:atomic} |{A: a[idx] := val; return true; }|;
